rocq-osiris/theories/program_logic/rules/record_rules.v
@@ -1,0 +1,179 @@
+From iris Require Import gen_heap proofmode.proofmode.
+From osiris Require Import lang type_nel.
+From osiris.tactics Require Import osiris_utils.
+From osiris.program_logic Require Import ewp.
+From osiris.program_logic.rules Require Import impure_rules stop_rules.
+From osiris.logic Require Import list_z big_opLZ.
+
+(** This file defines record resource predicates and [imp] rules for record expressions. *)
+
+Section record_resources.
+
+  Context `{!osirisGS Σ}.
+
+  Fixpoint to_vals {τ : types} : τ-#> list val :=
+    match τ with
+    | Tbase H => tbind (λ x, [ #x])
+    | @type_nel.Tcons X H b =>
+      λ (x : X), @tbind _ b (λ tt, #x :: (to_vals tt))
+    end.
+
+  Fixpoint length (τ : types) : Z :=
+    match τ with
+    | Tbase _ => 1
+    | type_nel.Tcons _ τ => 1 + length τ
+    end.
+
+  Lemma to_vals_length (τ : types) :
+    ∀ (xs : τ), list_z.length (to_vals xs) = length τ.
+  Proof.
+    induction τ.
+    - intros x. simpl. unfold tapp. by rewrite length_singleton.
+    - intros (x & xs). simpl. rewrite tapp_bind. length.
+      rewrite IHτ. lia.
+  Qed.
+
+  Definition ownRecord {τ : types} (r : record) dq (t : mut_tag) (xs : τ) : iProp Σ :=
+    ∃ ls, isBlockLocs r ls ∗ r ⤇{dq} t ∗
+      [∗ listZ] l;v ∈ ls; (to_vals xs), l ↦{dq} v.
+
+End record_resources.
+
+Section records_reasoning.
+
+  Context `{!osirisGS Σ}.
+
+  Context {η : env} {E : coPset} {Ψ : iEff Σ}.
+
+  Lemma imp_as_record {ζ} {Φ : record → iProp Σ} (m : microvx) :
+    imp m @ E <|Ψ|> ⟨⟨ ζ ⟩⟩ {{ Φ }} -∗
+    impure E (as_record m) Ψ ζ Φ.
+  Proof.
+    iIntros "Hm".
+    iApply (imp_bind with "Hm").
+    iIntros (r) "HΦ".
+    iApply (imp_ret with "HΦ"). encode.
+  Qed.
+
+  Global Instance observe_types (τ : types) : Observe τ (list val) :=
+    { observe τ := to_vals τ }.
+
+  Global Instance notval_listloc : NotVal (list loc) := {}.
+  Local Instance notval_listval : NotVal (list val) := {}.
+
+  Lemma imp_ERecord {τ : types} {ζ} (Φs : τ -#> iProp Σ) t es :
+    ⌜length τ ≤ max_array_length⌝ -∗
+    impure E (evals η es) Ψ ζ Φs -∗
+    impure E (eval η (ERecord t es)) Ψ ζ
+      (λ r, ∃ (xs : τ), ownRecord r (DfracOwn 1) t xs ∗ Φs xs).
+  Proof.
+    iIntros "%Hlength Hes". simpl_eval.
+    iApply (imp_bind with "Hes").
+    iIntros (xs) "HΦs".
+    iApply imp_bind.
+    { simpl.
+      replace (to_vals xs) with
+      (@observe (list val) (list val) (@observe_list val Encode_val) (to_vals xs)).
+      iApply (@imp_allocn _ _ _ _ _ val Encode_val (λ ls, [∗ listZ] l;v ∈ ls; (to_vals xs), l ↦ v)%I (to_vals xs)).
+      iIntros "!>" (ls) "$".
+      simpl. rewrite map_id. reflexivity. }
+    iIntros (ls) "Hls".
+    iPoseProof (big_sepLZ2_length with "Hls") as "%Hlength_ls".
+    iApply imp_bind.
+    { iApply imp_alloc_block.
+      iPureIntro. simpl.
+      rewrite Hlength_ls. rewrite to_vals_length. assumption. }
+    iIntros (r) "(Hmut & Hblocks)".
+    iApply imp_ret. encode.
+    iFrame.
+  Qed.
+
+  Instance types_lookup : Lookup Z Type types :=
+    λ i xs, if decide (i < 0) then None else
+      let fix go (i : nat) (τ : types) {struct τ} : option Type :=
+        match τ, i with
+        | Tbase X, 1%nat => Some X
+        | Tbase _, _ => None
+        | type_nel.Tcons X _, 0%nat => Some X
+        | type_nel.Tcons _ τ, (S i0) => go i0 τ
+        end
+        in
+      go (Z.to_nat i) xs.
+
+  Instance types_lookup_total : LookupTotal Z Type types :=
+    λ i xs, if decide (i < 0) then ()%type else
+      let fix go (i : nat) (τ : types) {struct τ} : Type :=
+        match τ, i with
+        | Tbase X, 1%nat => X
+        | Tbase _, _ => unit
+        | type_nel.Tcons X _, 0%nat => X
+        | type_nel.Tcons _ τ, (S i0) => go i0 τ
+        end
+      in
+      go (Z.to_nat i) xs.
+
+  Definition types_go : nat -> types -> Type :=
+    fix go (i : nat) (τ : types) {struct τ} : Type :=
+      match τ, i with
+      | Tbase X, 1%nat => X
+      | Tbase _, _ => unit
+      | type_nel.Tcons X _, 0%nat => X
+      | type_nel.Tcons _ τ', S i0 => go i0 τ'
+      end.
+
+  Fixpoint tau_lookup_go (τ : types) (i : nat) : τ -> types_go i τ :=
+    match τ, i return τ -> types_go i τ with
+    | Tbase X, 1%nat => fun xs => xs
+    | Tbase _, _ => fun _ => tt
+    | type_nel.Tcons X _, 0%nat => fun xs => fst xs
+    | type_nel.Tcons _ τ', S i0 => fun xs => tau_lookup_go τ' i0 (snd xs)
+    end.
+
+  Definition τ_lookup_total {τ : types} (f : Z) (xs : τ) : τ !!! f.
+  Proof.
+    unfold lookup_total, types_lookup_total.
+    case_decide.
+    - exact tt.
+    - exact (tau_lookup_go τ (Z.to_nat f) xs).
+  Defined.
+
+  Notation "xs !!τ f" := (τ_lookup_total f xs) (at level 20).
+
+  Global Instance encode_types_lookup {τ : types} {f : Z} : Encode (τ !!! f).
+  Proof.
+    unfold lookup_total, types_lookup_total.
+    case_decide. { apply _. }
+    generalize (Z.to_nat f).
+    induction τ; intros n.
+    - destruct n as [|[|]]; apply _.
+    - destruct n.
+      + destruct τ0; apply _.
+      + apply IHτ.
+  Qed.
+
+  Global Instance notval_block : NotVal (mut_tag * list loc) := {}.
+
+  Lemma imp_ERecordAccess {τ : types} {ζ} f {Φ : (τ !!! f) → iProp Σ} r ls e :
+    ▷ isBlockLocs r ls -∗
+    impure E (eval η e) Ψ ζ (λ (r' : record), ⌜r' = r⌝) -∗
+    (∃ dq t (xs : τ),
+      ▷ ownRecord r dq t xs ∗
+      ▷ (ownRecord r dq t xs -∗ Φ (xs !!τ f))) -∗
+    impure E (eval η (ERecordAccess e f)) Ψ ζ Φ.
+  Proof.
+    iIntros "#Hblock He P". simpl_eval.
+    iApply (imp_bind with "[He]").
+    { iApply (imp_as_record with "He"). }
+    iIntros (?) "->".
+    iDestruct "P" as
+        "(%dq & %t & %xs & P)".
+    rewrite <- (bi.later_sep (ownRecord _ _ _ _)).
+
+
+    iApply (imp_bind (A1:=(mut_tag * list loc)) with "[P]").
+    { iApply (imp_load_block_ghost' with "Hblock P"). }
+    iIntros ((? & ?)) "(-> & Hown & HΦ) /=".
+
+    Admitted.
+
+End records_reasoning.
